begin inference definition

Wasm_Big_Step.thy
@@ -103,4 +103,142 @@ inductive reduce_to :: "[(s \<times> v list \<times> e list), (nat list \<times>
 | label_return:"\<lbrakk>(s,vs,es) \<Down>{(n#ls,r,i)} (s',vs',RReturn rvs)\<rbrakk> \<Longrightarrow> (s,vs,[Label n les es]) \<Down>{(ls,r,i)} (s',vs',RReturn rvs)"
 | local_return:"\<lbrakk>(s,lls,es) \<Down>{([],n,j)} (s',lls',RReturn rvs)\<rbrakk> \<Longrightarrow> (s,vs,[Local n j lls es]) \<Down>{\<Gamma>} (s',vs,RValue rvs)"
 
+inductive reduce_to_n :: "[(s \<times> v list \<times> e list), nat, (nat list \<times> nat \<times> inst), (s \<times> v list \<times> res_b)] \<Rightarrow> bool" ("_ \<Down>_{_} _" 60) where
+  \<comment> \<open>\<open>constant values\<close>\<close>
+  const:"(s,vs,[$C v]) \<Down>k{\<Gamma>} (s,vs,RValue [v])"
+  \<comment> \<open>\<open>unary ops\<close>\<close>
+| unop:"(s,vs,[$C v, $(Unop t op)]) \<Down>k{\<Gamma>} (s,vs,RValue [(app_unop op v)])"
+  \<comment> \<open>\<open>binary ops\<close>\<close>
+| binop_Some:"\<lbrakk>app_binop op v1 v2 = (Some v)\<rbrakk> \<Longrightarrow> (s,vs,[$C v1, $C v2, $(Binop t op)]) \<Down>k{\<Gamma>} (s,vs,RValue [v])"
+| binop_None:"\<lbrakk>app_binop op v1 v2 = None\<rbrakk> \<Longrightarrow> (s,vs,[$C v1, $C v2, $(Binop t op)]) \<Down>k{\<Gamma>} (s,vs,RTrap)"
+  \<comment> \<open>\<open>testops\<close>\<close>
+| testop:"(s,vs,[$C v, $(Testop t op)]) \<Down>k{\<Gamma>} (s,vs,RValue [(app_testop op v)])"
+  \<comment> \<open>\<open>relops\<close>\<close>
+| relop:"(s,vs,[$C v1, $C v2, $(Relop t op)]) \<Down>k{\<Gamma>} (s,vs,RValue [(app_relop op v1 v2)])"
+  \<comment> \<open>\<open>convert\<close>\<close>
+| convert_Some:"\<lbrakk>types_agree t1 v; cvt t2 sx v = (Some v')\<rbrakk> \<Longrightarrow> (s,vs,[$(C v), $(Cvtop t2 Convert t1 sx)]) \<Down>k{\<Gamma>} (s,vs,RValue [v'])"
+| convert_None:"\<lbrakk>types_agree t1 v; cvt t2 sx v = None\<rbrakk> \<Longrightarrow> (s,vs,[$(C v), $(Cvtop t2 Convert t1 sx)]) \<Down>k{\<Gamma>} (s,vs,RTrap)"
+  \<comment> \<open>\<open>reinterpret\<close>\<close>
+| reinterpret:"types_agree t1 v \<Longrightarrow> (s,vs,[$(C v), $(Cvtop t2 Reinterpret t1 None)]) \<Down>k{\<Gamma>} (s,vs,RValue [(wasm_deserialise (bits v) t2)])"
+  \<comment> \<open>\<open>unreachable\<close>\<close>
+| unreachable:"(s,vs,[$ Unreachable]) \<Down>k{\<Gamma>} (s,vs,RTrap)"
+  \<comment> \<open>\<open>nop\<close>\<close>
+| nop:"(s,vs,[$ Nop]) \<Down>k{\<Gamma>} (s,vs,RValue [])"
+  \<comment> \<open>\<open>drop\<close>\<close>
+| drop:"(s,vs,[$(C v), ($ Drop)]) \<Down>k{\<Gamma>} (s,vs,RValue [])"
+  \<comment> \<open>\<open>select\<close>\<close>
+| select_false:"int_eq n 0 \<Longrightarrow> (s,vs,[$(C v1), $(C v2), $C (ConstInt32 n), ($ Select)]) \<Down>k{\<Gamma>} (s,vs, RValue [v2])"
+| select_true:"int_ne n 0 \<Longrightarrow> (s,vs,[$(C v1), $(C v2), $C (ConstInt32 n), ($ Select)]) \<Down>k{\<Gamma>} (s,vs,RValue [v1])"
+  \<comment> \<open>\<open>block\<close>\<close>
+| block:"\<lbrakk>const_list ves; length ves = n; length t1s = n; length t2s = m; (s,vs,[Label m [] (ves @ ($* es))]) \<Down>k{\<Gamma>} (s',vs',res)\<rbrakk> \<Longrightarrow> (s,vs,ves @ [$(Block (t1s _> t2s) es)]) \<Down>k{\<Gamma>} (s',vs',res)"
+  \<comment> \<open>\<open>loop\<close>\<close>
+| loop:"\<lbrakk>const_list ves; length ves = n; length t1s = n; length t2s = m; (s,vs,[Label n [] (ves @ ($* es))]) \<Down>k{\<Gamma>} (s',vs',res)\<rbrakk> \<Longrightarrow> (s,vs,ves @ [$(Loop (t1s _> t2s) es)]) \<Down>k{\<Gamma>} (s',vs',res)"
+  \<comment> \<open>\<open>if\<close>\<close>
+| if_false:"\<lbrakk>int_eq n 0; const_list ves; (s,vs,ves@[$(Block tf e2s)]) \<Down>k{\<Gamma>} (s',vs',res)\<rbrakk> \<Longrightarrow> (s,vs,ves@[$C (ConstInt32 n), $(If tf e1s e2s)]) \<Down>k{\<Gamma>} (s',vs',res)"
+| if_true:"\<lbrakk>int_ne n 0; const_list ves; (s,vs,ves@[$(Block tf e1s)]) \<Down>k{\<Gamma>} (s',vs',res)\<rbrakk> \<Longrightarrow> (s,vs,ves@[$C (ConstInt32 n), $(If tf e1s e2s)]) \<Down>k{\<Gamma>} (s',vs',res)"
+  \<comment> \<open>\<open>br\<close>\<close>
+| br:"\<lbrakk>length vcs = n; j < length ls; ls!j = n\<rbrakk> \<Longrightarrow> (s,vs,(($$*vcs) @ [$(Br j)])) \<Down>k{(ls,r,i)} (s,vs,RBreak j vcs)"
+  \<comment> \<open>\<open>br_if\<close>\<close>
+| br_if_false:"int_eq n 0 \<Longrightarrow> (s,vs,[$C (ConstInt32 n), $(Br_if j)]) \<Down>k{\<Gamma>} (s,vs,RValue [])"
+| br_if_true:"\<lbrakk>int_ne n 0; const_list ves; (s,vs,ves@[$(Br j)]) \<Down>k{\<Gamma>} (s',vs',res) \<rbrakk> \<Longrightarrow> (s,vs,ves@[$C (ConstInt32 n), $(Br_if j)]) \<Down>k{\<Gamma>} (s',vs',res)"
+  \<comment> \<open>\<open>br_table\<close>\<close>
+| br_table:"\<lbrakk>length js > (nat_of_int c); const_list ves; (s,vs,ves@[$(Br (js!(nat_of_int c)))]) \<Down>k{\<Gamma>} (s',vs',res)\<rbrakk> \<Longrightarrow> (s,vs,ves@[$C (ConstInt32 c), $(Br_table js j)]) \<Down>k{\<Gamma>} (s',vs',res)"
+| br_table_length:"\<lbrakk>length js \<le> (nat_of_int c); const_list ves; (s,vs,ves@[$(Br j)]) \<Down>k{\<Gamma>} (s',vs',res)\<rbrakk> \<Longrightarrow> (s,vs,ves@[$C (ConstInt32 c), $(Br_table js j)]) \<Down>k{\<Gamma>} (s',vs',res)"
+  \<comment> \<open>\<open>return\<close>\<close>
+| return:"\<lbrakk>length vs = r\<rbrakk>  \<Longrightarrow> (s,vs,($$*vcs) @ [$Return]) \<Down>k{(ls,r,i)} (s',vs',RReturn vcs)"
+  \<comment> \<open>\<open>get_local\<close>\<close>
+| get_local:"\<lbrakk>length vi = j\<rbrakk> \<Longrightarrow> (s,(vi @ [v] @ vs),[$(Get_local j)]) \<Down>k{\<Gamma>} (s,(vi @ [v] @ vs),RValue [v])"
+  \<comment> \<open>\<open>set_local\<close>\<close>
+| set_local:"\<lbrakk>length vi = j\<rbrakk> \<Longrightarrow> (s,(vi @ [v] @ vs),[$(C v'), $(Set_local j)]) \<Down>k{\<Gamma>} (s,(vi @ [v'] @ vs),RValue [])"
+  \<comment> \<open>\<open>tee_local\<close>\<close>
+| tee_local:"\<lbrakk>is_const v; (s,vs,[v, v, $(Set_local i)]) \<Down>k{\<Gamma>} (s',vs',res)\<rbrakk> \<Longrightarrow> (s,vs,[v, $(Tee_local i)]) \<Down>k{\<Gamma>} (s',vs',res)"
+  \<comment> \<open>\<open>get_global\<close>\<close>
+| get_global:"(s,vs,[$(Get_global j)]) \<Down>k{(ls,r,i)} (s,vs,RValue [(sglob_val s i j)])"
+  \<comment> \<open>\<open>set_global\<close>\<close>
+| set_global:"supdate_glob s i j v = s' \<Longrightarrow> (s,vs,[$(C v), $(Set_global j)]) \<Down>k{(ls,r,i)} (s',vs,RValue [])"
+  \<comment> \<open>\<open>load\<close>\<close>
+| load_Some:"\<lbrakk>smem_ind s i = Some j; ((mem s)!j) = m; load m (nat_of_int n) off (t_length t) = Some bs\<rbrakk> \<Longrightarrow> (s,vs,[$C (ConstInt32 n), $(Load t None a off)]) \<Down>k{(ls,r,i)} (s,vs,RValue [(wasm_deserialise bs t)])"
+| load_None:"\<lbrakk>smem_ind s i = Some j; ((mem s)!j) = m; load m (nat_of_int n) off (t_length t) = None\<rbrakk> \<Longrightarrow> (s,vs,[$C (ConstInt32 n), $(Load t None a off)]) \<Down>k{(ls,r,i)} (s,vs,RTrap)"
+  \<comment> \<open>\<open>load packed\<close>\<close>
+| load_packed_Some:"\<lbrakk>smem_ind s i = Some j; ((mem s)!j) = m; load_packed sx m (nat_of_int n) off (tp_length tp) (t_length t) = Some bs\<rbrakk> \<Longrightarrow> (s,vs,[$C (ConstInt32 n), $(Load t (Some (tp, sx)) a off)]) \<Down>k{(ls,r,i)} (s,vs,RValue [(wasm_deserialise bs t)])"
+| load_packed_None:"\<lbrakk>smem_ind s i = Some j; ((mem s)!j) = m; load_packed sx m (nat_of_int n) off (tp_length tp) (t_length t) = None\<rbrakk> \<Longrightarrow> (s,vs,[$C (ConstInt32 n), $(Load t (Some (tp, sx)) a off)]) \<Down>k{(ls,r,i)} (s,vs,RTrap)"
+  \<comment> \<open>\<open>store\<close>\<close>
+| store_Some:"\<lbrakk>types_agree t v; smem_ind s i = Some j; ((mem s)!j) = m; store m (nat_of_int n) off (bits v) (t_length t) = Some mem'\<rbrakk> \<Longrightarrow> (s,vs,[$C (ConstInt32 n), $C v, $(Store t None a off)]) \<Down>k{(ls,r,i)} (s\<lparr>mem:= ((mem s)[j := mem'])\<rparr>,vs,RValue [])"
+| store_None:"\<lbrakk>types_agree t v; smem_ind s i = Some j; ((mem s)!j) = m; store m (nat_of_int n) off (bits v) (t_length t) = None\<rbrakk> \<Longrightarrow> (s,vs,[$C (ConstInt32 n), $C v, $(Store t None a off)]) \<Down>k{(ls,r,i)} (s,vs,RTrap)"
+  \<comment> \<open>\<open>store packed\<close>\<close> (* take only (tp_length tp) lower order bytes *)
+| store_packed_Some:"\<lbrakk>types_agree t v; smem_ind s i = Some j; ((mem s)!j) = m; store_packed m (nat_of_int n) off (bits v) (tp_length tp) = Some mem'\<rbrakk> \<Longrightarrow> (s,vs,[$C (ConstInt32 n), $C v, $(Store t (Some tp) a off)]) \<Down>k{(ls,r,i)} (s\<lparr>mem:= ((mem s)[j := mem'])\<rparr>,vs,RValue [])"
+| store_packed_None:"\<lbrakk>types_agree t v; smem_ind s i = Some j; ((mem s)!j) = m; store_packed m (nat_of_int n) off (bits v) (tp_length tp) = None\<rbrakk> \<Longrightarrow> (s,vs,[$C (ConstInt32 n), $C v, $(Store t (Some tp) a off)]) \<Down>k{(ls,r,i)} (s,vs,RTrap)"
+  \<comment> \<open>\<open>current_memory\<close>\<close>
+| current_memory:"\<lbrakk>smem_ind s i = Some j; ((mem s)!j) = m; mem_size m = n\<rbrakk> \<Longrightarrow> (s,vs,[ $(Current_memory)]) \<Down>k{(ls,r,i)} (s,vs,RValue [(ConstInt32 (int_of_nat n))])"
+  \<comment> \<open>\<open>grow_memory\<close>\<close>
+| grow_memory:"\<lbrakk>smem_ind s i = Some j; ((mem s)!j) = m; mem_size m = n; mem_grow m (nat_of_int c) = mem'\<rbrakk> \<Longrightarrow> (s,vs,[$C (ConstInt32 c), $(Grow_memory)]) \<Down>k{(ls,r,i)} (s\<lparr>mem:= ((mem s)[j := mem'])\<rparr>,vs, RValue [(ConstInt32 (int_of_nat n))])"
+  \<comment> \<open>\<open>grow_memory fail\<close>\<close>
+| grow_memory_fail:"\<lbrakk>smem_ind s i = Some j; ((mem s)!j) = m; mem_size m = n\<rbrakk> \<Longrightarrow> (s,vs,[$C (ConstInt32 c),$(Grow_memory)]) \<Down>k{(ls,r,i)} (s,vs,RValue [(ConstInt32 int32_minus_one)])"
+  \<comment> \<open>\<open>call\<close>\<close>
+| call:"\<lbrakk>const_list ves; (s,vs,ves@[Callcl (sfunc s i j)]) \<Down>k{(ls,r,i)} (s',vs',res)\<rbrakk> \<Longrightarrow> (s,vs,ves@[$(Call j)]) \<Down>k{(ls,r,i)} (s',vs',res)"
+  \<comment> \<open>\<open>call_indirect\<close>\<close>
+| call_indirect_Some:"\<lbrakk>stab s i (nat_of_int c) = Some cl; stypes s i j = tf; cl_type cl = tf; const_list ves; (s,vs,ves@[Callcl cl]) \<Down>{(ls,r,i)} (s',vs',res)\<rbrakk> \<Longrightarrow> (s,vs,ves@[$C (ConstInt32 c), $(Call_indirect j)]) \<Down>k{(ls,r,i)} (s',vs',res)"
+| call_indirect_None:"\<lbrakk>(stab s i (nat_of_int c) = Some cl \<and> stypes s i j \<noteq> cl_type cl) \<or> stab s i (nat_of_int c) = None\<rbrakk> \<Longrightarrow> (s,vs,[$C (ConstInt32 c), $(Call_indirect j)]) \<Down>k{(ls,r,i)} (s,vs,RTrap)"
+  \<comment> \<open>\<open>call\<close>\<close>
+| callcl_native:"\<lbrakk>cl = Func_native j (t1s _> t2s) ts es; ves = ($$* vcs); length vcs = n; length t1s = n; length t2s = m; (n_zeros ts = zs); (s,vs,[Local m j (vcs@zs) [$(Block ([] _> t2s) es)]]) \<Down>k{(ls,r,i)} (s',vs',res)\<rbrakk> \<Longrightarrow> (s,vs,ves @ [Callcl cl]) \<Down>(Suc k){(ls,r,i)} (s',vs',res)"
+| callcl_host_Some:"\<lbrakk>cl = Func_host (t1s _> t2s) f; ves = ($$* vcs); length vcs = n; length t1s = n; length t2s = m; host_apply s (t1s _> t2s) f vcs hs = Some (s', vcs')\<rbrakk> \<Longrightarrow> (s,vs,ves @ [Callcl cl]) \<Down>k{(ls,r,i)} (s',vs,RValue vcs')"
+| callcl_host_None:"\<lbrakk>cl = Func_host (t1s _> t2s) f; ves = ($$* vcs); length vcs = n; length t1s = n; length t2s = m\<rbrakk> \<Longrightarrow> (s,vs,ves @ [Callcl cl]) \<Down>k{(ls,r,i)} (s,vs,RTrap)"
+  \<comment> \<open>\<open>value congruence\<close>\<close>
+| seq_value:"\<lbrakk>(s,vs,es) \<Down>k{\<Gamma>} (s'',vs'',RValue res''); (s'',vs'',($$* res'') @ es') \<Down>k{\<Gamma>} (s',vs',RValue res)\<rbrakk> \<Longrightarrow> (s,vs,es @ es') \<Down>k{\<Gamma>} (s',vs',RValue res)"
+| label_value:"\<lbrakk>(s,vs,es) \<Down>k{(n#ls,r,i)} (s',vs',RValue res)\<rbrakk> \<Longrightarrow> (s,vs,[Label n les es]) \<Down>k{(ls,r,i)} (s',vs',RValue res)"
+| local_value:"\<lbrakk>(s,lls,es) \<Down>k{([],n,j)} (s',lls',RValue res)\<rbrakk> \<Longrightarrow> (s,vs,[Local n j lls es]) \<Down>k{\<Gamma>} (s',vs,RValue res)"
+  \<comment> \<open>\<open>trap congruence\<close>\<close>
+| seq_trap:"\<lbrakk>const_list ves; (s,vs,es) \<Down>k{\<Gamma>} (s',vs',RTrap)\<rbrakk> \<Longrightarrow> (s,vs,ves @ es @ es') \<Down>k{\<Gamma>} (s',vs',RTrap)"
+| label_trap:"\<lbrakk>(s,vs,es) \<Down>k{(n#ls,r,i)} (s',vs',RTrap)\<rbrakk> \<Longrightarrow> (s,vs,[Label n les es]) \<Down>k{(ls,r,i)} (s',vs',RTrap)"
+| local_trap:"\<lbrakk>(s,lls,es) \<Down>k{([],n,j)} (s',lls',RTrap)\<rbrakk> \<Longrightarrow> (s,vs,[Local n j lls es]) \<Down>k{\<Gamma>} (s',vs,RTrap)"
+  \<comment> \<open>\<open>break congruence\<close>\<close>
+| seq_break:"\<lbrakk>const_list ves; (s,vs,es) \<Down>k{\<Gamma>} (s',vs',RBreak n bvs)\<rbrakk> \<Longrightarrow> (s,vs,ves @ es @ es') \<Down>k{\<Gamma>} (s',vs',RBreak n bvs)"
+| label_break_suc:"\<lbrakk>(s,vs,es) \<Down>k{(n#ls,r,i)} (s',vs',RBreak (Suc bn) bvs)\<rbrakk> \<Longrightarrow> (s,vs,[Label n les es]) \<Down>k{(ls,r,i)} (s',vs',RBreak bn bvs)"
+| label_break_nil:"\<lbrakk>(s,vs,es) \<Down>k{(n#ls,r,i)} (s',vs',RBreak 0 bvs)\<rbrakk> \<Longrightarrow> (s,vs,[Label n les es]) \<Down>k{(ls,r,i)} (s',vs',RValue bvs)"
+  \<comment> \<open>\<open>return congruence\<close>\<close>
+| seq_return:"\<lbrakk>const_list ves; (s,vs,es) \<Down>k{\<Gamma>} (s',vs',RReturn rvs)\<rbrakk> \<Longrightarrow> (s,vs,ves @ es @ es') \<Down>k{\<Gamma>} (s',vs',RReturn rvs)"
+| label_return:"\<lbrakk>(s,vs,es) \<Down>k{(n#ls,r,i)} (s',vs',RReturn rvs)\<rbrakk> \<Longrightarrow> (s,vs,[Label n les es]) \<Down>k{(ls,r,i)} (s',vs',RReturn rvs)"
+| local_return:"\<lbrakk>(s,lls,es) \<Down>k{([],n,j)} (s',lls',RReturn rvs)\<rbrakk> \<Longrightarrow> (s,vs,[Local n j lls es]) \<Down>k{\<Gamma>} (s',vs,RValue rvs)"
+
+lemma reduce_to_n_mono:
+  assumes "(c1 \<Down>k{\<Gamma>} c2)"
+  shows"\<forall>k' \<ge> k. (c1 \<Down>k'{\<Gamma>} c2)"
+  using assms
+proof (induction rule: reduce_to_n.induct)
+  case (callcl_native cl j t1s t2s ts es ves vcs n m zs s vs k ls r i s' vs' res)
+  show ?case
+    using reduce_to_n.callcl_native[OF callcl_native(1,2,3,4,5,6)] callcl_native(8)
+    by (metis Suc_le_D Suc_le_lessD less_Suc_eq_le)
+qed (fastforce intro: reduce_to_n.intros)+
+
+lemma reduce_to_imp_reduce_to_n:
+  assumes "(c1 \<Down>{\<Gamma>} c2)"
+  shows"(\<exists>k. (c1 \<Down>k{\<Gamma>} c2))"
+  using assms
+proof (induction rule: reduce_to.induct)
+  case (callcl_native cl j t1s t2s ts es ves vcs n k m zs s vs ls r i s' vs' res)
+  show ?case
+    using reduce_to_n.callcl_native[OF callcl_native(1,2,3,5,6,7), of s vs _ ls r i s' vs' res]
+    callcl_native(9)
+    by auto
+next
+  case (seq_value s vs es \<Gamma> s'' vs'' res'' es' s' vs' res)
+  thus ?case
+    using reduce_to_n_mono reduce_to_n.seq_value
+    by (meson le_cases)
+qed (fastforce intro: reduce_to_n.intros)+
+
+lemma reduce_to_n_imp_reduce_to:
+  assumes "(c1 \<Down>k{\<Gamma>} c2)"
+  shows"(c1 \<Down>{\<Gamma>} c2)"
+  using assms
+  apply (induction rule: reduce_to_n.induct)
+                      apply (fastforce intro: reduce_to.intros)+
+  done
+
+lemma reduce_to_iff_reduce_to_n:
+  shows "(c1 \<Down>{\<Gamma>} c2) = (\<exists>k. (c1 \<Down>k{\<Gamma>} c2))"
+  using reduce_to_imp_reduce_to_n reduce_to_n_imp_reduce_to
+  by blast
+
 end
