Wasm_Assertions_Shallow.thy
@@ -1,31 +1,59 @@
-theory Wasm_Assertions_Shallow imports "WebAssembly/Wasm_Base_Defs" begin
+theory Wasm_Assertions_Shallow imports "Wasm_Big_Step" begin
 
 typedef lvar = "UNIV :: (nat) set" ..
 
 (* global, local, logical variables*)
 datatype var = Gl nat | Lc nat | Lv lvar
 
+datatype 'a lvar_v = V_p v | V_a 'a
+
 (* variable store *)
-type_synonym var_st = "(var, v) map"
+(* global, local, logical variables*)
+type_synonym 'a var_st = "global list \<times> v list \<times> (lvar, 'a lvar_v) map"
 
-definition var_st_locals :: "var_st \<Rightarrow> nat set" where
-  "var_st_locals st = {n. Lc n \<in> (dom st)}"
+definition var_st_get_local :: "'a var_st \<Rightarrow> nat \<Rightarrow> v option" where
+  "var_st_get_local st n \<equiv> let st_l = (fst (snd st)) in
+                            (if (n < length st_l)
+                            then Some (st_l!n)
+                            else None)"
 
-definition var_st_globals :: "var_st \<Rightarrow> nat set" where
-  "var_st_globals st = {n. Gl n \<in> (dom st)}"
+definition var_st_get_global :: "'a var_st \<Rightarrow> nat \<Rightarrow> global option" where
+  "var_st_get_global st n \<equiv> let st_g = (fst st) in
+                            (if (n < length st_g)
+                            then Some (st_g!n)
+                            else None)"
+
+definition var_st_set_lvar :: "'a var_st \<Rightarrow> lvar \<Rightarrow> 'a lvar_v \<Rightarrow> 'a var_st" where
+  "var_st_set_lvar st l lv \<equiv> let (gs, vs, lvs) = st in
+                              (gs, vs, (lvs(l \<mapsto> lv)))"
 
 (* abstract heap with max length *)
 type_synonym heap = "((nat, byte) map) \<times> (nat option)"
 
+definition map_disj :: "('a,'b) map \<Rightarrow> ('a,'b) map \<Rightarrow> bool" where
+  "map_disj m1 m2 \<equiv> Set.disjnt (dom m1) (dom m2)"
+
+definition option_disj :: "'a option \<Rightarrow> 'a option \<Rightarrow> bool" where
+  "option_disj o1 o2 \<equiv> Option.is_none o1 \<or> Option.is_none o2"
+
+definition heap_disj :: "heap \<Rightarrow> heap \<Rightarrow> bool" where
+  "heap_disj h1 h2 \<equiv> map_disj (fst h1) (fst h2) \<and> option_disj (snd h1) (snd h2)"
+
+definition heap_merge :: "heap \<Rightarrow> heap \<Rightarrow> heap" where
+  "heap_merge h1 h2 \<equiv> let (m1,s1) = h1 in
+                       let (m2,s2) = h2 in
+                       (m1 ++ m2, case_option s2 (\<lambda>s. Some s) s1)"
+
 (* local variable reification *)
-definition reifies_loc :: "[v list, var_st] \<Rightarrow> bool" where
-  "reifies_loc locs st \<equiv> \<forall>ln \<in> var_st_locals st. ln < (length locs) \<and> st (Lc ln) = Some (locs!ln)"
+definition reifies_loc :: "[v list, 'a var_st] \<Rightarrow> bool" where
+  "reifies_loc locs st \<equiv> (fst (snd st)) = locs"
 
 (* global variable reification (with respect to a partial instance) *)
-definition reifies_glob :: "[global list, nat list, var_st] \<Rightarrow> bool" where
+definition reifies_glob :: "[global list, nat list, 'a var_st] \<Rightarrow> bool" where
   "reifies_glob gs igs st \<equiv>
-     \<forall>gn \<in> var_st_globals st.
-       gn < (length igs) \<and> igs!gn < (length gs) \<and> st (Gl gn) = Some (g_val (gs!(igs!gn)))"
+     let st_g = (fst st) in
+     \<forall>gn < length st_g.
+       gn < (length igs) \<and> igs!gn < (length gs) \<and> st_g!gn = (gs!(igs!gn))"
 
 (* function reification (with respect to a partial instance) *)
 definition reifies_func :: "[cl list, nat list, cl list] \<Rightarrow> bool" where
@@ -46,8 +74,111 @@ definition reifies_heap :: "[mem list, nat option, heap] \<Rightarrow> bool" whe
                              \<and> reifies_heap_length (ms!im) (snd h)"
 
 (* store reification relation *)
-definition reifies_s :: "[s, inst, heap, var_st, cl list] \<Rightarrow> bool" where
+definition reifies_s :: "[s, inst, heap, 'a var_st, cl list] \<Rightarrow> bool" where
   "reifies_s s i h st fs \<equiv> reifies_glob (globs s) (inst.globs i) st
                          \<and> reifies_func (funcs s) (inst.funcs i) fs
                          \<and> reifies_heap (mem s) (inst.mem i) h"
+
+(* shallow embedding of assertions *)
+type_synonym 'a stack_ass = "(v \<Rightarrow> 'a var_st \<Rightarrow> bool) list"
+type_synonym 'a heap_ass = "heap \<Rightarrow> 'a var_st \<Rightarrow> bool"
+
+datatype 'a ass = Ass "'a stack_ass" "'a heap_ass" (infix "\<^sub>s|\<^sub>h" 60) | Ex_ass lvar "'a ass" 
+
+type_synonym 'a triple = "'a ass \<times> e list \<times> 'a ass"
+
+(* function list, assms, label ass, return ass *)
+type_synonym 'a triple_context = "cl list \<times> 'a ass list \<times> 'a ass"
+
+definition add_label_ass :: "'a triple_context \<Rightarrow> 'a ass \<Rightarrow> 'a triple_context" where
+  "add_label_ass \<Gamma> l \<equiv> let (fs, labs, ret) = \<Gamma> in (fs, l#labs, ret)"
+
+fun ass_sat :: "'a ass \<Rightarrow> v list \<Rightarrow> heap \<Rightarrow> 'a var_st \<Rightarrow> bool" where
+  "ass_sat (St \<^sub>s|\<^sub>h H) ves h st = (list_all2 (\<lambda>Si v. Si v st) St ves \<and> H h st)"
+| "ass_sat (Ex_ass lv P) ves h st = (\<exists>v. ass_sat P ves h (var_st_set_lvar st lv v))"
+
+fun ass_stack_len :: "'a ass \<Rightarrow> nat" where
+  "ass_stack_len (St \<^sub>s|\<^sub>h H) = length St"
+| "ass_stack_len (Ex_ass lv P) = ass_stack_len P"
+
+(* label reification relation *)
+definition reifies_lab :: "nat list \<Rightarrow> 'a triple_context \<Rightarrow> bool" where
+  "reifies_lab lns \<Gamma> \<equiv> lns = map ass_stack_len (fst (snd \<Gamma>))"
+
+(* label reification relation *)
+definition reifies_ret :: "nat \<Rightarrow> 'a triple_context \<Rightarrow> bool" where
+  "reifies_ret rn \<Gamma> \<equiv> rn = ass_stack_len (snd (snd \<Gamma>))"
+
+(* TODO: frame? ? ? ?*)
+definition valid_triple :: "'a triple_context \<Rightarrow> 'a ass \<Rightarrow> e list \<Rightarrow> 'a ass \<Rightarrow> bool" ("_ \<Turnstile> {_}_{_}" 60) where
+  "(\<Gamma> \<Turnstile> {P}es{Q}) \<equiv> let (fs,lasss,rass) = \<Gamma> in
+                     \<forall>vcs h st s i locs labs ret lvar_st.
+                                        ass_sat P vcs h st
+                                      \<and> reifies_s s i h st fs
+                                      \<and> reifies_loc locs st
+                                      \<and> reifies_lab labs \<Gamma>
+                                      \<and> reifies_ret ret \<Gamma>
+                                      \<and> snd (snd st) = lvar_st \<longrightarrow>
+                                      (\<forall>s' locs' res. ((s,locs,($$*vcs)@es) \<Down>{(labs,ret,i)} (s',locs', res)) \<longrightarrow>
+                                      (case res of
+                                         RTrap \<Rightarrow> False
+                                       | RValue rvs \<Rightarrow> \<exists>h' vcs' st'.
+                                                               ass_sat Q vcs' h' st'
+                                                               \<and> rvs = vcs'
+                                                               \<and> reifies_s s' i h' st' fs
+                                                               \<and> reifies_loc locs' st'
+                                       | RBreak n rvs \<Rightarrow> \<exists>h' vcs' st'.
+                                                               n < length lasss
+                                                               \<and> ass_sat (lasss!n) vcs' h' st'
+                                                               \<and> rvs = vcs'
+                                                               \<and> reifies_s s' i h' st' fs
+                                                               \<and> reifies_loc locs' st'
+                                       | RReturn rvs \<Rightarrow> \<exists>h' vcs' st'.
+                                                               ass_sat rass vcs' h' st'
+                                                               \<and> rvs = vcs'
+                                                               \<and> reifies_s s' i h' st' fs
+                                                               \<and> reifies_loc locs' st'))"
+
+definition valid_triples :: "'a triple_context \<Rightarrow> 'a triple set \<Rightarrow> bool" ("_ \<TTurnstile> _" 60) where
+  "\<Gamma> \<TTurnstile> specs \<equiv> \<forall>(P,es,Q) \<in> specs. (\<Gamma> \<Turnstile> {P}es{Q})"
+
+(* TODO: frame? ? ? ?*)
+definition valid_triple_n :: "'a triple_context \<Rightarrow> nat \<Rightarrow> 'a ass \<Rightarrow> e list \<Rightarrow> 'a ass \<Rightarrow> bool" ("_ \<Turnstile>\<^sub>_ {_}_{_}" 60) where
+  "(\<Gamma> \<Turnstile>\<^sub>k {P}es{Q}) \<equiv> let (fs,lasss,rass) = \<Gamma> in
+                     \<forall>vcs h st s i locs labs ret lvar_st.
+                                        ass_sat P vcs h st
+                                      \<and> reifies_s s i h st fs
+                                      \<and> reifies_loc locs st
+                                      \<and> reifies_lab labs \<Gamma>
+                                      \<and> reifies_ret ret \<Gamma>
+                                      \<and> snd (snd st) = lvar_st \<longrightarrow>
+                                      (\<forall>s' locs' res. ((s,locs,($$*vcs)@es)\<Down>k{(labs,ret,i)} (s',locs', res)) \<longrightarrow>
+                                      (case res of
+                                         RTrap \<Rightarrow> False
+                                       | RValue rvs \<Rightarrow> \<exists>h' vcs' st'.
+                                                               ass_sat Q vcs' h' st'
+                                                               \<and> rvs = vcs'
+                                                               \<and> reifies_s s' i h' st' fs
+                                                               \<and> reifies_loc locs' st'
+                                       | RBreak n rvs \<Rightarrow> \<exists>h' vcs' st'.
+                                                               n < length lasss
+                                                               \<and> ass_sat (lasss!n) vcs' h' st'
+                                                               \<and> rvs = vcs'
+                                                               \<and> reifies_s s' i h' st' fs
+                                                               \<and> reifies_loc locs' st'
+                                       | RReturn rvs \<Rightarrow> \<exists>h' vcs' st'.
+                                                               ass_sat rass vcs' h' st'
+                                                               \<and> rvs = vcs'
+                                                               \<and> reifies_s s' i h' st' fs
+                                                               \<and> reifies_loc locs' st'))"
+
+definition valid_triples_n :: "'a triple_context \<Rightarrow> nat \<Rightarrow> 'a triple set \<Rightarrow> bool" ("_ \<TTurnstile>\<^sub>_ _" 60) where
+  "(\<Gamma> \<TTurnstile>\<^sub>n specs) \<equiv> \<forall>(P,es,Q) \<in> specs. (\<Gamma> \<Turnstile>\<^sub>n {P}es{Q})"
+
+definition cvalids :: "'a triple_context \<Rightarrow> 'a triple set \<Rightarrow> 'a triple set \<Rightarrow> bool" ("_\<bullet>_ \<TTurnstile> _" 60) where
+  "(\<Gamma>\<bullet>assms \<TTurnstile> specs) \<equiv> (\<Gamma> \<TTurnstile> assms) \<longrightarrow> (\<Gamma> \<TTurnstile> specs)"
+
+definition cvalids_n :: "'a triple_context \<Rightarrow> 'a triple set \<Rightarrow> nat \<Rightarrow> 'a triple set \<Rightarrow> bool" ("_\<bullet>_ \<TTurnstile>\<^sub>_ _" 60) where
+  "(\<Gamma>\<bullet>assms \<TTurnstile>\<^sub>n specs) \<equiv> (\<Gamma> \<TTurnstile>\<^sub>n assms) \<longrightarrow> (\<Gamma> \<TTurnstile>\<^sub>n specs)"
+
 end
