WebAssembly/Wasm_Axioms.thy
@@ -2,39 +2,44 @@ section {* Host Properties *}
 
 theory Wasm_Axioms imports Wasm begin
 
+lemma old_mem_size_def:
+  shows "mem_size m = length (Rep_mem m) div Ki64"
+  unfolding mem_size_def mem_length_def
+  by simp
+
 (* these were originally axioms, but memory now has a concrete representation in the model *)
 lemma mem_grow_size:
   assumes "mem_grow m n = m'"
-  shows "(mem_size m + (Ki64 * n)) = mem_size m'"
+  shows "(mem_size m + n) = mem_size m'"
   using assms Abs_mem_inverse Abs_bytes_inverse
-  unfolding mem_grow_def mem_size_def mem_append_def bytes_replicate_def
-  by auto
+  unfolding mem_grow_def old_mem_size_def mem_append_def bytes_replicate_def
+  by (auto simp add: Ki64_def)
 
 lemma load_size:
-  "(load m n off l = None) = (mem_size m < (off + n + l))"
+  "(load m n off l = None) = (mem_length m < (off + n + l))"
   unfolding load_def
-  by (cases "n + off + l \<le> mem_size m") auto
+  by (cases "n + off + l \<le> mem_length m") auto
 
 lemma load_packed_size:
-  "(load_packed sx m n off lp l = None) = (mem_size m < (off + n + lp))"
+  "(load_packed sx m n off lp l = None) = (mem_length m < (off + n + lp))"
   using load_size
   unfolding load_packed_def
-  by (cases "n + off + l \<le> mem_size m") auto  
+  by (cases "n + off + l \<le> mem_length m") auto  
 
 lemma store_size1:
-  "(store m n off v l = None) = (mem_size m < (off + n + l))"
+  "(store m n off v l = None) = (mem_length m < (off + n + l))"
   unfolding store_def
-  by (cases "n + off + l \<le> mem_size m") auto
+  by (cases "n + off + l \<le> mem_length m") auto
 
 lemma store_size:
   assumes "(store m n off v l = Some m')"
   shows "mem_size m = mem_size m'"
-  using assms Abs_mem_inverse Abs_bytes_inverse
+  using assms Abs_mem_inverse Abs_bytes_inverse mem_length.rep_eq
   unfolding store_def write_bytes_def bytes_takefill_def
-  by (cases "n + off + l \<le> mem_size m") (auto simp add: mem_size_def)
+  by (cases "n + off + l \<le> mem_length m") (auto simp add: old_mem_size_def)
 
 lemma store_packed_size1:
-  "(store_packed m n off v l = None) = (mem_size m < (off + n + l))"
+  "(store_packed m n off v l = None) = (mem_length m < (off + n + l))"
   using store_size1
   unfolding store_packed_def
   by simp
